cleaning

code/ecdsap256/Hacl.Impl.P256.Core.fsti
@@ -23,7 +23,7 @@ module B = LowStar.Buffer
 open FStar.Mul
 
 
-#set-options "--z3rlimit 200" 
+#set-options "--z3rlimit 50" 
 
 inline_for_extraction noextract 
 val toDomain: #c: curve -> value: felem c -> result: felem c ->  Stack unit 
@@ -99,15 +99,7 @@ val normX: #c: curve -> p: point c -> result: felem c
     let (xN, _, _) = _norm #c (pxD, pyD, pzD) in 
     as_nat c h1 result == xN))
 
-val lemma_sm: #c: curve -> p: point c -> h: mem -> Lemma
-  (requires (point_eval c h p))
-  (ensures (
-    let prime = getPrime c in 
-    let len = v (getCoordinateLenU64 c) in 
-    felem_seq_as_nat c (Lib.Sequence.sub (as_seq h p) 0 len) < prime /\
-    felem_seq_as_nat c (Lib.Sequence.sub (as_seq h p) len len) < prime /\
-    felem_seq_as_nat c (Lib.Sequence.sub (as_seq h p) (len * 2) len) < prime))
-
+#push-options "--z3rlimit 100" 
 
 inline_for_extraction noextract
 val scalarMultiplication: #c: curve -> #buf_type: buftype->  p: point c -> result: point c 
@@ -119,13 +111,12 @@ val scalarMultiplication: #c: curve -> #buf_type: buftype->  p: point c -> resul
     LowStar.Monotonic.Buffer.all_disjoint [loc p; loc tempBuffer; loc scalar; loc result] /\ 
     point_eval c h p)
   (ensures fun h0 _ h1 -> 
-    point_eval c h0 p /\ 
+    point_eval c h0 p /\
     point_eval c h1 result /\
     modifies (loc p |+| loc result |+| loc tempBuffer) h0 h1 /\ (
-    let x3, y3, z3 = point_x_as_nat c h1 result, point_y_as_nat c h1 result, point_z_as_nat c h1 result in 
-    lemma_sm #c p h0; 
-    let (xN, yN, zN) = scalar_multiplication #c (as_seq h0 scalar) (point_prime_to_coordinates c (as_seq h0 p)) in 
-    x3 == xN /\ y3 == yN /\ z3 == zN 
+    let r = point_prime_to_coordinates c (as_seq h1 result) in
+    let rN = scalar_multiplication #c (as_seq h0 scalar) (point_prime_to_coordinates c (as_seq h0 p)) in 
+    r == rN
   ))
 
 
@@ -134,23 +125,12 @@ val scalarMultiplicationWithoutNorm: #c: curve -> p: point c -> result: point c 
   tempBuffer: lbuffer uint64 (size 20 *! getCoordinateLenU64 c) ->
   Stack unit
     (requires fun h -> 
-      let prime = getPrime c in 
-      let len = getCoordinateLenU64 c in
-    
+      point_eval c h p /\
       live h p /\ live h result /\ live h scalar /\ live h tempBuffer /\
-      LowStar.Monotonic.Buffer.all_disjoint [loc p; loc tempBuffer; loc scalar; loc result] /\
-      as_nat c h (gsub p (size 0) len) < prime /\ 
-      as_nat c h (gsub p len len) < prime /\
-      as_nat c h (gsub p (size 2 *! len) len) < prime
+      LowStar.Monotonic.Buffer.all_disjoint [loc p; loc tempBuffer; loc scalar; loc result]
     )
   (ensures fun h0 _ h1 -> 
-    let prime = getPrime c in 
-    let len = getCoordinateLenU64 c in
-    
-    as_nat c h1 (gsub result (size 0) len) < prime /\ 
-    as_nat c h1 (gsub result len len) < prime /\
-    as_nat c h1 (gsub result (size 2 *! len) len) < prime /\
-    
+    point_eval c h1 result /\
     modifies (loc p |+| loc result |+| loc tempBuffer) h0 h1 /\
     (
       let p1 = fromDomainPoint #c (point_prime_to_coordinates c (as_seq h1 result)) in 
@@ -168,19 +148,13 @@ val secretToPublic: #c: curve -> result: point c  -> scalar: lbuffer uint8 (getS
       LowStar.Monotonic.Buffer.all_disjoint [loc tempBuffer; loc scalar; loc result]
     )
   (ensures fun h0 _ h1 -> 
-    let prime = getPrime c in 
-    let len = getCoordinateLenU64 c in
-    
-    modifies (loc result |+| loc tempBuffer) h0 h1 /\
-    
-    as_nat c h1 (gsub result (size 0) len) < prime /\ 
-    as_nat c h1 (gsub result len len) < prime /\ 
-    as_nat c h1 (gsub result (size 2 *! len) len) < prime /\
+    point_eval c h0 result /\
+    modifies (loc result |+| loc tempBuffer) h0 h1 (* /\
     (
-      let x3, y3, z3 = point_x_as_nat c h1 result, point_y_as_nat c h1 result, point_z_as_nat c h1 result in 
+      let x3, y3, z3 = point_prime_to_coordinates
       let (xN, yN, zN) = secret_to_public #c (as_seq h0 scalar)  in 
       x3 == xN /\ y3 == yN /\ z3 == zN 
-    )
+    ) *)
   )
 
 val secretToPublicWithoutNorm: #c: curve -> result: point c -> scalar: lbuffer uint8 (getScalarLen c) -> 
