code/ecdsap256/Hacl.Impl.ECDSA.P256.Verification.Agile.fst
@@ -264,7 +264,7 @@ val ecdsa_verification_step5_0:
       let fromDomainPointU1 = fromDomainPoint #c (point_prime_to_coordinates c (as_seq h1 pointU1)) in
       let fromDomainPointU2 = fromDomainPoint #c (point_prime_to_coordinates c (as_seq h1 pointU2)) in
       let pointAtInfinity = (0, 0, 0) in
-      let u1D, _ = montgomery_ladder_spec #P256 (as_seq h0 u1) (pointAtInfinity, basePoint) in
+      let u1D, _ = montgomery_ladder_spec #P256 (as_seq h0 u1) (pointAtInfinity, basePoint #c) in
       let u2D, _ = montgomery_ladder_spec #P256 (as_seq h0 u2) (pointAtInfinity, point_prime_to_coordinates c (as_seq h0 pubKeyAsPoint)) in
       fromDomainPointU1 == u1D /\ fromDomainPointU2 == u2D
     )
@@ -304,10 +304,10 @@ val ecdsa_verification_step5_1:
       as_nat c h1 (gsub pointSum (size 0) (size 4)) < prime256 /\
       (
         let pointAtInfinity = (0, 0, 0) in
-        let u1D, _ = montgomery_ladder_spec (as_seq h0 u1) (pointAtInfinity, basePoint #P256) in
-        let u2D, _ = montgomery_ladder_spec (as_seq h0 u2) (pointAtInfinity, point_prime_to_coordinates c (as_seq h0 pubKeyAsPoint)) in
-        let sumD = _point_add u1D u2D in
-        let pointNorm = _norm sumD in
+        let u1D, _ = montgomery_ladder_spec #c (as_seq h0 u1) (pointAtInfinity, basePoint #P256) in
+        let u2D, _ = montgomery_ladder_spec #c (as_seq h0 u2) (pointAtInfinity, point_prime_to_coordinates c (as_seq h0 pubKeyAsPoint)) in
+        let sumD = _point_add #c u1D u2D in
+        let pointNorm = _norm #c sumD in
         let resultPoint =  point_prime_to_coordinates c (as_seq h1 pointSum) in
         pointNorm == resultPoint
       )
@@ -353,10 +353,10 @@ val ecdsa_verification_step5:
       as_nat c h1 x < prime256 /\
       (
         let pointAtInfinity = (0, 0, 0) in
-        let u1D, _ = montgomery_ladder_spec (as_seq h0 u1) (pointAtInfinity, basePoint #P256) in
-        let u2D, _ = montgomery_ladder_spec (as_seq h0 u2) (pointAtInfinity, point_prime_to_coordinates c (as_seq h0 pubKeyAsPoint)) in
-        let sumD = _point_add u1D u2D in
-        let pointNorm = _norm sumD in
+        let u1D, _ = montgomery_ladder_spec #c (as_seq h0 u1) (pointAtInfinity, basePoint #c) in
+        let u2D, _ = montgomery_ladder_spec #c (as_seq h0 u2) (pointAtInfinity, point_prime_to_coordinates c (as_seq h0 pubKeyAsPoint)) in
+        let sumD = _point_add #c u1D u2D in
+        let pointNorm = _norm #c sumD in
         let (xResult, yResult, zResult) = pointNorm in
         state == not (Spec.P256.isPointAtInfinity pointNorm) /\
         as_nat c h1 x == xResult
@@ -448,11 +448,11 @@ val ecdsa_verification_core:
 	 let bufferU1 = nat_to_bytes_be 32 p0  in 
 	 let bufferU2 = nat_to_bytes_be 32 p1 in 
 	 let pointAtInfinity = (0, 0, 0) in
-         let u1D, _ = montgomery_ladder_spec bufferU1 (pointAtInfinity, basePoint #P256) in
-         let u2D, _ = montgomery_ladder_spec bufferU2 (pointAtInfinity, point_prime_to_coordinates c (as_seq h0 publicKeyPoint)) in
-         let sumD = _point_add u1D u2D in
-         let (xResult, yResult, zResult) = _norm sumD in
-         state == not (Spec.P256.isPointAtInfinity (_norm sumD)) /\
+         let u1D, _ = montgomery_ladder_spec #c bufferU1 (pointAtInfinity, basePoint #P256) in
+         let u2D, _ = montgomery_ladder_spec #c bufferU2 (pointAtInfinity, point_prime_to_coordinates c (as_seq h0 publicKeyPoint)) in
+         let sumD = _point_add #c u1D u2D in
+         let (xResult, yResult, zResult) = _norm #c sumD in
+         state == not (Spec.P256.isPointAtInfinity (_norm #c sumD)) /\
          as_nat c h1 xBuffer == xResult
       )
   )
