code/ecdsap256/Hacl.P256.fst
@@ -79,7 +79,8 @@ let ecp256dh_i result scalar = Hacl.Impl.P256.DH.ecp256dh_i P256 result scalar
 
 let ecp384dh_i result scalar = Hacl.Impl.P256.DH.ecp256dh_i P384 result scalar
 
-
+(* 
 
 let ecp256dh_r result pubKey scalar = Hacl.Impl.P256.DH.ecp256dh_r P256 result pubKey scalar
 
+ *)
